src-lite/decl_worklist.v
@@ -1,9 +1,5 @@
 Require Export bidir.notations.
 
-Notation "k $ e" :=
-  (open_dworklist_wrt_bexpr k e)
-    (at level 57, left associativity) : dworklist_scope.
-
 Reserved Notation "G1 ⫢ G2" (at level 58, left associativity).
 Fixpoint dwl_app (G1 G2 : dworklist) :=
   match G2 with
@@ -34,20 +30,33 @@ Fixpoint to_bctx (Γ : dworklist) : bcontext :=
   end
 where "⌊ wl ⌋" := (to_bctx wl) : bcontext_scope.
 
+Inductive apply_dcont : dcont → bexpr → dworklist → Prop :=
+| apdc_done : forall e, apply_dcont dc_done e dwl_nil
+| apdc_app : forall A e1 e2 c,
+  apply_dcont (dc_app e1 e2 c) A (dwl_nil ⊨ A ⋅ e1 & e2 ⇒ c)
+| apdc_reduce : forall A c,
+  apply_dcont (dc_reduce c) A (dwl_nil ⊨ A ⟼ c)
+| apdc_check : forall A B,
+  apply_dcont (dc_check B) A (dwl_nil ⊨ A ≲ B)
+| apdc_inst : forall A B c k,
+  apply_dcont (dc_inst B c) A (dwl_nil ⊨ c $ A ⊨ A <: B ⇐ ⧼k⧽')
+.
+
 Reserved Notation "⪧ wl" (at level 60, no associativity).
 Inductive dwl_step : dworklist → Prop :=
 | dst_nil : ⪧ dwl_nil
 | dst_infer : forall Γ e1 e2 c A
   , ⌊ Γ ⌋ ⊢ e1 <: e2 ⇒ A
-  → ⪧ Γ ⫢ c $ A
+  → ⪧ Γ ⊨ c $ A
   → ⪧ Γ ⊨ e1 <: e2 ⇒ c
-| dst_infer_app : forall Γ A e c B
-  , ⌊ Γ ⌋ ⊢ A ⋅ e ⇒ B
-  → ⪧ Γ ⫢ c $ B
-  → ⪧ Γ ⊨ A ⋅ e ⇒ c
+| dst_infer_app : forall Γ A c e1 e2 B C
+  , ⌊ Γ ⌋ ⊢ A ⇒Π B, C
+  → ⌊ Γ ⌋ ⊢ e1 <: e2 ⇐ B
+  → ⪧ Γ ⊨ c $ B ^^' e1
+  → ⪧ Γ ⊨ A ⋅ e1 & e2 ⇒ c
 | dst_reduce : forall Γ A c B
   , ⌊ Γ ⌋ ⊢ A ⟼ B
-  → ⪧ Γ ⫢ c $ B
+  → ⪧ Γ ⊨ c $ B
   → ⪧ Γ ⊨ A ⟼ c
 | dst_comp : forall Γ A B k
   , ⌊ Γ ⌋ ⊢ A <: B ⇒ ⧼ k ⧽'
@@ -57,8 +66,12 @@ Inductive dwl_step : dworklist → Prop :=
   , ⪧ Γ
   → ⪧ Γ ⊨ ◻' ≲ ◻'
 | dst_check : forall Γ ob e1 e2 A
-  , ⪧ Γ ,? ob ⊨ e1 <: e2 ⇒ (dwl_nil ⊨ ↑'0 ≲ A)
+  , ⪧ Γ ,? ob ⊨ e1 <: e2 ⇒ dc_check A
   → ⪧ Γ ⊨ ob ⊢? e1 <: e2 ⇐ A
+| dst_app_cont : forall Γ c e Γ'
+  , apply_dcont c e Γ'
+  → ⪧ Γ ⫢ Γ'
+  → ⪧ Γ ⊨ c $ e
 where "⪧ wl" := (dwl_step wl) : type_scope
 .
 
