src-lite/wl_properties.v
@@ -39,29 +39,11 @@ Proof.
   - admit.
   (* num *)
   - destruct IHwl_step as (Γ0 & Θ & Inst & DeclSolve).
-    apply inst_wl_split in Inst as (Γ1 & Γ2 & Θ0 & -> & Inst1 & Inst2).
-    pick fresh x for (fv_worklist c `union` fv_ss Θ).
-    rewrite (subst_worklist_intro x) in Inst2; auto.
-    assert (exists Θ', Θ0 ;; Θ' = Θ) as (Θ' & <-)
-        by eauto using inst_wl_ss_extend.
-    eapply inst_wl_rev_subst with (e := be_int) in Inst2
-        as (c' & Θ'' & <- & <- & Inst2).
-    exists (Γ1 ⊨ be_num n ⇒ close_dworklist_wrt_bexpr x c'). exists (Θ0 ;; Θ'') (* todo *).
-    split.
-    + apply instwl_cons with Θ0.
-      * auto.
-      * eapply instw_infer; eauto. intros.
-        rewrite (subst_worklist_intro x).
-        rewrite (subst_dworklist_intro x).
-        apply inst_wl_rename.
-        rewrite open_dworklist_wrt_bexpr_close_dworklist_wrt_bexpr. auto.
-        all: admit.
-    + eapply dst_infer with be_int.
-      * admit.
-      * now rewrite <- subst_dworklist_spec.
-    + admit.
-    + admit.
-    + admit.
+    inversion Inst; subst.
+    inversion H6; subst.
+    exists (Γ1 ⊨ be_num n ⇒ c0), Θ; split.
+    + now constructor.
+    + econstructor. 2: eauto. admit.
   (* int *)
   - admit.
   (* star *)
@@ -71,12 +53,7 @@ Proof.
   (* bot check *)
   - admit.
   (* app *)
-  - destruct IHwl_step as (Γ' & Θ & Inst & Solve).
-    dependent destruction Inst.
-    dependent destruction H0.
-    dependent destruction Solve.
-
-    admit.
+  - admit.
   (* lambda check *)
   - admit.
   (* pi *)
@@ -90,25 +67,15 @@ Proof.
     dependent destruction Inst.
     dependent destruction H0. dependent destruction H0.
     dependent destruction H4. dependent destruction H4.
-    apply inst_wl_split in Inst as (Γ1 & Γ2 & Θ' & -> & Inst1 & Inst2).
-    dependent destruction Inst1.
-    pick fresh x' for all.
-    rewrite (subst_worklist_intro x) in Inst2.
-    assert (exists Θ'0, Θ' ; x1 ≔ ⧼k0⧽ ;; Θ'0 = Θ) as (Θ'0 & <-)
-        by eauto using inst_wl_ss_extend.
-    eapply inst_wl_rev_subst with (e := ⧼k0⧽') in Inst2
-        as (c_' & Θ'0' & <- & <- & Inst2).
-    exists (Γ0 ⊨ be_pi A0 (close_bexpr_wrt_bexpr x e1) <: be_pi A4 (close_bexpr_wrt_bexpr x e0) ⇒ (close_dworklist_wrt_bexpr x c_')), nil. split.
+
+    dependent destruction Inst.
+    dependent destruction Inst.
+    dependent destruction H1.
+    dependent destruction H12.
+    dependent destruction H12.
+
+    dependent destruction Solve.
     all: admit.
-    (*
-    + admit.
-    + eapply dst_infer with (⧼k0⧽').
-      dependent destruction H10.
-      dependent destruction H10.
-      assert (A5 = ⧼k0⧽') as -> by admit.
-      assert (e4 = e5) as -> by admit.
-      all: admit.
-    *)
   (* bind check *)
   - admit.
   (* forall L *)
