src-lite/worklist.v
@@ -1,9 +1,5 @@
 Require Export alg.notations.
 
-Notation "k $′ e" :=
-  (open_worklist_wrt_aexpr k e)
-    (at level 57, left associativity) : worklist_scope.
-
 Reserved Notation "G1 ⫢′ G2" (at level 58, left associativity).
 Fixpoint wl_app (G1 G2 : worklist) :=
   match G2 with
@@ -116,22 +112,22 @@ Inductive monoize : atoms → aexpr → vsign → aexpr → list binding → Pro
 | mz_ex    : forall x s L, `^x  ⤚ s ⇥ `^x  ‖ nil \ L
 | mz_num : forall n s L, ae_num n ⤚ s ⇥ ae_num n ‖ nil \ L
 | mz_int : forall   s L, ae_int   ⤚ s ⇥ ae_int   ‖ nil \ L
-| mz_bot : forall s ψ L
-  , ae_bot ⤚ s ⇥ ae_bot ‖ ψ \ L
+| mz_bot : forall s ψ L A
+  , ae_bot A ⤚ s ⇥ ae_bot A ‖ ψ \ L
 | mz_app : forall f1 f2 a s ψ L
   , mono_atype a
   → f1 ⤚ s ⇥ f2 ‖ ψ \ L
   → ae_app f1 a ⤚ s ⇥ ae_app f2 a ‖ ψ \ L
-| mz_abs : forall e1 e2 s ψ L
+| mz_abs : forall e1 A B e2 s ψ L
   , e1 ⤚ s ⇥ e2 ‖ ψ \ L
-  → λ′ e1 ⤚ s ⇥ λ′ e2 ‖ ψ \ L
+  → λ′ A , e1 : B ⤚ s ⇥ λ′ A , e2 : B ‖ ψ \ L
 | mz_pi : forall A1 A2 B1 B2 s ψ1 ψ2 L
   , A1 ⤚ (vneg s) ⇥ A2 ‖ ψ1 \ L
   → B1 ⤚ s ⇥ B2 ‖ ψ2 \ L
   → ae_pi A1 B1 ⤚ s ⇥ ae_pi A2 B2 ‖ ψ1 ++ ψ2 \ L
-| mz_bind : forall e1 e2 s ψ L
+| mz_bind : forall e1 A B e2 s ψ L
   , e1 ⤚ s ⇥ e2 ‖ ψ \ L
-  → Λ′ e1 ⤚ s ⇥ Λ′ e2 ‖ ψ \ L
+  → Λ′ A , e1 : B ⤚ s ⇥ Λ′ A , e2 : B ‖ ψ \ L
 | mz_forall_pos : forall L A B C ψ x
   , x `notin` L
   → B ^^′ `^x ⤚ ⊕ ⇥ C ‖ ψ \ add x L
@@ -143,13 +139,28 @@ Inductive monoize : atoms → aexpr → vsign → aexpr → list binding → Pro
 | mz_castdn : forall e1 e2 s ψ L
   , e1 ⤚ s ⇥ e2 ‖ ψ \ L
   → ae_castdn e1 ⤚ s ⇥ ae_castdn e2 ‖ ψ \ L
-| mz_castup : forall e1 e2 s ψ L
+| mz_castup : forall e1 A e2 s ψ L
   , e1 ⤚ s ⇥ e2 ‖ ψ \ L
-  → ae_castup e1 ⤚ s ⇥ ae_castup e2 ‖ ψ \ L
+  → ae_castup A e1 ⤚ s ⇥ ae_castup A e2 ‖ ψ \ L
 | mz_anno : forall e1 e2 A s ψ L
   , e1 ⤚ s ⇥ e2 ‖ ψ \ L
   → ae_anno e1 A ⤚ s ⇥ ae_anno e2 A ‖ ψ \ L
 where "e1 ⤚ s ⇥ e2 ‖ bs \ L" := (monoize L e1 s e2 bs) : type_scope.
+
+Inductive apply_cont : cont → aexpr → worklist → Prop :=
+| apc_app : forall c F e1 e2,
+  apply_cont (c_app e1 e2 c) F (wl_nil ⊨′ F ⋅ e1 & e2 ⇒′ c)
+| apc_reduce : forall c A,
+  apply_cont (c_reduce c) A (wl_nil ⊨′ A ⟼′ c)
+| apc_done : forall e,
+  apply_cont c_done e wl_nil
+| apc_check : forall A B,
+  apply_cont (c_check B) A (wl_nil ⊨′ A ≲′ B)
+| apc_inst : forall A B c k L
+  , k `notin` L (* ????????????? *)
+  → apply_cont (c_inst B c) A (wl_nil ⊨′ c $′ B ,′ ⧼^k⧽ ⊨′ A <: B ⇐′ ⧼`^k⧽)
+.
+
 
 #[export]
 Hint Constructors monoize : core.
@@ -198,26 +209,32 @@ Inductive syn_eq : aexpr → aexpr → Prop :=
 | seq_kind : forall k1 k2, kind_syn_eq k1 k2 → ⧼k1⧽′ ≃ ⧼k2⧽′
 | seq_num  : forall n, ae_num n ≃ ae_num n
 | seq_int  : ae_int ≃ ae_int
-| seq_bot  : ae_bot ≃ ae_bot
+| seq_bot  : forall A1 A2, A1 ≃ A2 → ae_bot A1 ≃ ae_bot A2
 | seq_app : forall f1 f2 a1 a2
   , f1 ≃ f2
   → a1 ≃ a2
   → ae_app f1 a2 ≃ ae_app f2 a2
-| seq_abs : forall L e1 e2
+| seq_abs : forall L e1 A1 A2 B1 B2 e2
   , (forall x, x `notin` L → e1 ^`′ x ≃ e2 ^`′ x)
-  → ae_abs e1 ≃ ae_abs e2
+  → (forall x, x `notin` L → B1 ^`′ x ≃ B2 ^`′ x)
+  → A1 ≃ A2
+  → λ′ A1, e1 : B1 ≃ λ′ A2, e2 : B2
 | seq_pi : forall L A1 A2 B1 B2
   , A1 ≃ A2
   → (forall x, x `notin` L → B1 ^`′ x ≃ B2 ^`′ x)
   → ae_pi A1 B1 ≃ ae_pi A2 B2
-| seq_bind : forall L e1 e2
+| seq_bind : forall L e1 A1 A2 B1 B2 e2
   , (forall x, x `notin` L → e1 ^`′ x ≃ e2 ^`′ x)
-  → ae_bind e1 ≃ ae_bind e2
+  → (forall x, x `notin` L → B1 ^`′ x ≃ B2 ^`′ x)
+  → A1 ≃ A2
+  → Λ′ A1 , e1 : B1 ≃ Λ′ A1 , e1 : B1
 | seq_all : forall L A1 A2 B1 B2
   , A1 ≃ A2
   → (forall x, x `notin` L → B1 ^`′ x ≃ B2 ^`′ x)
   → ae_all A1 B1 ≃ ae_all A2 B2
-| seq_castup : forall e1 e2 , e1 ≃ e2 → ae_castup e1 ≃ ae_castup e2
+| seq_castup : forall e1 A1 A2 e2
+  , e1 ≃ e2 → A1 ≃ A2
+    → ae_castup A1 e1 ≃ ae_castup A2 e2
 | seq_castdn : forall e1 e2 , e1 ≃ e2 → ae_castdn e1 ≃ ae_castdn e2
 | seq_anno : forall e1 e2 A1 A2
   , e1 ≃ e2 → A1 ≃ A2
@@ -225,85 +242,94 @@ Inductive syn_eq : aexpr → aexpr → Prop :=
 where "e1 ≃ e2" := (syn_eq e1 e2) : type_scope
 .
 
-
 Reserved Notation "⪧′ wl" (at level 65, no associativity).
 Inductive wl_step : worklist -> Prop :=
 | st_nil : ⪧′ wl_nil
 (* decl-like inference *)
 | st_var : forall Γ x A c
   , x :′ A  ∈′ Γ
-  → ⪧′ Γ ⫢′ c $′ A
+  → ⪧′ Γ ⊨′ c $′ A
   → ⪧′ Γ ⊨′ `′ x ⇒′ c
 | st_num : forall Γ n c
-  , ⪧′ Γ ⫢′ c $′ ae_int
+  , ⪧′ Γ ⊨′ c $′ ae_int
   → ⪧′ Γ ⊨′ ae_num n ⇒′ c
 | st_int : forall Γ c
-  , ⪧′ Γ ⫢′ c $′ ⋆′
+  , ⪧′ Γ ⊨′ c $′ ⋆′
   → ⪧′ Γ ⊨′ ae_int ⇒′ c
 | st_star_inf : forall Γ c
-  , ⪧′ Γ ⫢′ c $′ ◻′
+  , ⪧′ Γ ⊨′ c $′ ◻′
   → ⪧′ Γ ⊨′ ⋆′ ⇒′ c
 | st_star_chk : forall Γ
   , ⪧′ Γ
   → ⪧′ Γ ⊨′ ⋆′ ⇐′ ◻′
-| st_bot : forall L Γ b A
-  , (forall k, k `notin` L -> ⪧′ Γ ,?′ b ,′ ⧼^k ⧽ ⊨′ A ⇐′ ⧼`^k⧽)
-  → ⪧′ Γ ⊨′ b ⊢? ae_bot <: ae_bot ⇐′ A
-| st_app : forall Γ f1 f2 a1 a2 c
-  , ⪧′ Γ ⊨′ f1 <: f2 ⇒′ ⦃ ↑′0 ⋅ a1 & a2 ⇒′ c ⦄
+| st_bot : forall L Γ A1 A2 c
+  , (forall k, k `notin` L
+    -> ⪧′ Γ ,′ ⧼^k⧽ ⊨′ A1 <: A2 ⇐′ ⧼`^k⧽ ⊨′ A2 <: A1 ⇐′ ⧼`^k⧽)
+  → ⪧′ Γ ⊨′ c $′ A1 ⊨′ ae_bot A1 <: ae_bot A2 ⇒′ c
+| st_app : forall Γ L f1 f2 a1 a2 c
+  , smono_atype a1 → smono_atype a2
+  → (forall k, k `notin` L →
+      ⪧′ Γ ⊨′ f1 <: f2 ⇒′ c_app a1 a2 c)
   -> ⪧′ Γ ⊨′ ae_app f1 a1 <: ae_app f2 a2 ⇒′ c
-| st_abs : forall L Γ b e1 e2 A B
+| st_abs : forall L Γ e1 e2 A1 A2 B1 B2 c
   , (forall x, x `notin` L → forall k1, k1 `notin` add x L
     → forall k2, k2 `notin` add k1 (add x L)
-      → ⪧′ Γ ,?′ b ,′ ⧼^k2⧽ ⊨′ A ⇐′ ⧼`^k1⧽
-      ⊨′ x :?′ A ⊢? B ^`′ x ⇐′ ⧼`^k2⧽
-      ⊨′ x :?′ A ⊢? e1 ^`′ x <: e2 ^`′ x ⇐′ B ^`′ x)
-  → ⪧′ Γ ⊨′ b ⊢? λ′ e1 <: λ′ e2 ⇐′ ae_pi A B
+      → ⪧′ Γ ⊨′ c $′ ae_pi A1 B1 ,′ ⧼^k1⧽ ,′ ⧼^k2⧽
+      ⊨′ A1 <: A2 ⇐′ ⧼`^k1⧽ ⊨′ A2 <: A1 ⇐′ ⧼`^k1⧽
+      ⊨′ x :?′ A1 ⊢? B1 ^`′ x <: B2 ^`′ x ⇐′ ⧼`^k2⧽
+      ⊨′ x :?′ A1 ⊢? B2 ^`′ x <: B1 ^`′ x ⇐′ ⧼`^k2⧽
+      ⊨′ x :?′ A1 ⊢? e1 ^`′ x <: e2 ^`′ x ⇐′ B1 ^`′ x)
+  → ⪧′ Γ ⊨′ λ′ A1 , e1 : B1 <: λ′ A1 , e2 : B2 ⇒′ c
 | st_pi : forall L Γ A1 A2 B1 B2 c
   , (forall x, x `notin` L → forall k1, k1 `notin` add x L
     → forall k2, k2 `notin` add k1 (add x L)
-    → ⪧′ Γ ,′ ⧼^k2⧽ ⫢′ c $′ ⧼`^k2⧽
+    → ⪧′ Γ ,′ ⧼^k2⧽ ⊨′ c $′ ⧼`^k2⧽
       ⊨′ x :?′ A1 ⊢? B1 ^`′ x ⇐′ ⧼`^k2⧽
       ⊨′ x :?′ A2 ⊢? B1 ^`′ x <: B2 ^`′ x ⇐′ ⧼`^k2⧽
       ,′ ⧼^k1⧽ ⊨′ A2 <: A2 ⇐′ ⧼`^k1⧽)
   → ⪧′ Γ ⊨′ ae_pi A1 B1 <: ae_pi A2 B2 ⇒′ c
-| st_bind : forall L Γ b A B e1 e2 c
+| st_bind : forall L Γ A1 A2 B1 B2 e1 e2 c
   , (forall x, x `notin` L → forall k1, k1 `notin` add x L
     → forall k2, k2 `notin` add k1 (add x L)
-    → ⪧′ Γ ,?′ b ,′ ⧼^k2⧽ ⊨′ A ⇐′ ⧼`^k1⧽
-      ⊨′ x :?′ A ⊢? B ^`′ x ⇐′ ⧼`^k2⧽
-      ⊨′ x :?′ A ⊢? e1 ^`′ x <: e2 ^`′ x ⇐′ B ^`′ x)
-  → ⪧′ Γ ⊨′ b ⊢? Λ′ e1 <: Λ′ e2 ⇐′ c
+      → ⪧′ Γ ⊨′ c $′ ae_all A1 B1 ,′ ⧼^k1⧽ ,′ ⧼^k2⧽
+      ⊨′ A1 <: A2 ⇐′ ⧼`^k1⧽ ⊨′ A2 <: A1 ⇐′ ⧼`^k1⧽
+      ⊨′ x :?′ A1 ⊢? B1 ^`′ x <: B2 ^`′ x ⇐′ ⧼`^k2⧽
+      ⊨′ x :?′ A1 ⊢? B2 ^`′ x <: B1 ^`′ x ⇐′ ⧼`^k2⧽
+      ⊨′ x :?′ A1 ⊢? e1 ^`′ x <: e2 ^`′ x ⇐′ B1 ^`′ x)
+  → ⪧′ Γ ⊨′ Λ′ A1, e1 : B1 <: Λ′ A2 , e2 : B2 ⇒′ c
 | st_forall_l : forall L Γ A B C c
   , (forall x, x `notin` L → forall k, k `notin` add x L
     → forall t, t `notin` add k (add x L)
-    → ⪧′ Γ ⫢′ c $′ ⋆′ ,′ ⧼^k⧽ ⊨′ A ⇐′ ⧼`^k⧽
+    → ⪧′ Γ ⊨′ c $′ ⋆′ ,′ ⧼^k⧽ ⊨′ A ⇐′ ⧼`^k⧽
       ⊨′ x :?′ A ⊢? B ^`′ x ⇐′ ⧼`^k⧽
       ,′ ^t :′ A ⊨′ B ^^′ `^t <: C ⇐′ ⋆′)
   → ⪧′ Γ ⊨′ ae_all A B <: C ⇒′ c
 | st_forall_r : forall L Γ A B C c
   , (forall x, x `notin` L → forall k, k `notin` add x L
-    → ⪧′ Γ ⫢′ c $′ ⋆′ ,′ ⧼^k⧽ ⊨′ B ⇐′ ⧼`^k⧽
+    → ⪧′ Γ ⊨′ c $′ ⋆′ ,′ ⧼^k⧽ ⊨′ B ⇐′ ⧼`^k⧽
       ⊨′ x :?′ B ⊢? A <: C ^`′ x ⇐′ ⧼`^k⧽ ⊨′ A ⇐′ ⋆′)
   → ⪧′ Γ ⊨′ A <: ae_all B C ⇒′ c
 | st_forall : forall L Γ A1 A2 B C c
   , (forall x, x `notin` L → forall k, k `notin` add x L
-    → ⪧′ Γ ⫢′ c $′ ⋆′ ,′ ⧼^k⧽
+    → ⪧′ Γ ⊨′ c $′ ⋆′ ,′ ⧼^k⧽
       ⊨′ A1 ⇐′ ⧼`^k⧽ ⊨′ A2 ⇐′ ⧼`^k⧽
       ⊨′ x :?′ A1 ⊢? B ⇐′ ⋆′
       ⊨′ x :?′ A2 ⊢? ae_all A1 B <: C ^`′ x ⇐′ ⋆′)
   → ⪧′ Γ ⊨′ ae_all A1 B <: ae_all A2 C ⇒′ c
 | st_castdn : forall Γ e1 e2 c
-  , ⪧′ Γ ⊨′ e1 <: e2 ⇒′ ⦃ ↑′0 ⟼′ c ⦄
+  , ⪧′ Γ ⊨′ e1 <: e2 ⇒′ c_reduce c
   → ⪧′ Γ ⊨′ ae_castdn e1 <: ae_castdn e2 ⇒′ c
-| st_castup : forall L Γ A e1 e2 B
-  , A ⟶′ B
+| st_castup : forall L Γ A1 A2 e1 e2 B c
+  , A1 ⟶′ B
+  → A2 ⟶′ B
   → (forall k, k `notin` L
-    → ⪧′ Γ ,′ ⧼^k ⧽ ⊨′ A ⇐′ ⧼`^k⧽ ⊨′ e1 <: e2 ⇐′ B)
-  → ⪧′ Γ ⊨′ ae_castup e1 <: ae_castup e2 ⇐′ A
+    → ⪧′ Γ ,′ ⧼^k ⧽
+      ⊨′ A1 <: A2 ⇐′ ⧼`^k⧽ ⊨′ A2 <: A1 ⇐′ ⧼`^k⧽
+      ⊨′ e1 <: e2 ⇐′ B)
+  → ⪧′ Γ ⊨′ ae_castup A1 e1 <: ae_castup A2 e2 ⇒′ c
 | st_anno : forall L Γ e1 e2 A1 A2 c
   , (forall k, k `notin` L
-    → ⪧′ Γ ⫢′ c $′ A1 ,′ ⧼^k⧽
+    → ⪧′ Γ ⊨′ c $′ A1 ,′ ⧼^k⧽
       ⊨′ A1 <: A2 ⇐′ ⧼`^k⧽ ⊨′ A2 <: A2 ⇐′ ⧼`^k⧽
       ⊨′ e1 <: e2 ⇐′ A1)
   → ⪧′ Γ ⊨′ e1 ::′ A1 <: e2 ::′ A2 ⇒′ c
@@ -311,49 +337,44 @@ Inductive wl_step : worklist -> Prop :=
 (* ex vars *)
 | st_ex_eq : forall Γ x A c
   , ^x :′ A  ∈′ Γ
-  → ⪧′ Γ ⫢′ c $′ A
+  → ⪧′ Γ ⊨′ c $′ A
   → ⪧′ Γ ⊨′ `^x <: `^x ⇒′ c
 | st_ex_l : forall L Γ Γ' x A e e' ψ c
   , ^x :′ A  ∈′ Γ → `^x <> e
   → e ⤚ ⊖ ⇥ e' ‖ ψ \ L
   → Γ ⫢′ to_wl ψ ‖ nil ⊢ ^x ≔ e' ⊣ Γ'
-  → (forall k, k `notin` L `union` psi_dom ψ
-    → ⪧′ ⟦e' /′ ^x⟧ Γ'
-      ⊨′ e' <: e ⇒′ (⟦e' /′ ^x⟧ c ,′ ⧼^k⧽ ⊨′ ↑′0 <: A ⇐′ ⧼`^k⧽))
+  → ⪧′ ⟦e' /′ ^x⟧ Γ' ⊨′ e' <: e ⇒′ c_inst A (ex_subst_cont e' x c)
+      (* ⟦e' /′ ^x⟧ c ,′ ⧼^k⧽ ⊨′ ↑′0 <: A ⇐′ ⧼`^k⧽ *)
   → ⪧′ Γ ⊨′ `^x <: e ⇒′ c
 | st_ex_r : forall L Γ Γ' x A e e' ψ c
   , ^x :′ A  ∈′ Γ → `^x <> e
   → e ⤚ ⊕ ⇥ e' ‖ ψ \ L
   → Γ ⫢′ to_wl ψ ‖ nil ⊢ ^x ≔ e' ⊣ Γ'
-  → (forall k, k `notin` L `union` psi_dom ψ
-    → ⪧′ ⟦e' /′ ^x⟧ Γ'
-      ⊨′ e <: e' ⇒′ (⟦e' /′ ^x⟧ c ,′ ⧼^k⧽ ⊨′ ↑′0 <: A ⇐′ ⧼`^k⧽))
+  → ⪧′ ⟦e' /′ ^x⟧ Γ' ⊨′ e <: e' ⇒′ c_inst A (ex_subst_cont e' x c)
+     (* (⟦e' /′ ^x⟧ c ,′ ⧼^k⧽ ⊨′ ↑′0 <: A ⇐′ ⧼`^k⧽) *)
   → ⪧′ Γ ⊨′ e <: `^x ⇒′ c
 
 (* infer_app *)
 | st_iapp_forall : forall L Γ A B e1 e2 c
   , (forall x, x `notin` L → forall y, y `notin` add x L
-    → ⪧′ Γ ⊨′ x :?′ A ⊢? B ^`′ x ⇐′ ⋆′ ,′ ^y :′ A
-      ⊨′ B ^^′ `^y ⋅ e1 & e2 ⇒′ c)
+    → ⪧′ Γ ,′ ^y :′ A ⊨′ B ^^′ `^y ⋅ e1 & e2 ⇒′ c)
   → ⪧′ Γ ⊨′ ae_all A B ⋅ e1 & e2 ⇒′ c
 | st_iapp_pi : forall L Γ A B e1 e2 c
-  , mono_atype e1 → mono_atype e2 → e1 ≃ e2
-  → (forall x, x `notin` L → forall k, k `notin` add x L
-    → ⪧′ Γ ⫢′ c $′ B ^^′ e1 ⊨′ e1 <: e2 ⇐′ A ⊨′ e2 <: e1 ⇐′ A
-      ,′ ⧼^k⧽ ⊨′ x :?′ A ⊢? B ⇐′ ⧼`^k⧽)
+  , (forall x, x `notin` L → forall k, k `notin` add x L
+    → ⪧′ Γ ⊨′ c $′ B ^^′ e1 ⊨′ e1 <: e2 ⇐′ A)
   → ⪧′ Γ ⊨′ ae_pi A B ⋅ e1 & e2 ⇒′ c
-| st_iapp_ex : forall L Γ x e1 e2 c Γ1 Γ2
+| st_iapp_ex : forall L Γ x c Γ1 Γ2
   , Γ = Γ1 ,′ ^x :′ ⋆′ ⫢′ Γ2
   → (forall A, A `notin` L → forall B, B `notin` add A L
     → forall k, k `notin` add A (add B L) → forall F, F = ae_pi `^A `^B
     → ⪧′ Γ1 ,′ ⧼^k⧽ ,′ ^A :′ ⧼`^k⧽ ,′ ^B :′ ⋆′ ⫢′ ⟦ F /′ ^x ⟧ Γ2
-      ⊨′ F ⋅ [F /^ x ] e1 & [F /^ x] e2 ⇒′ ⟦ F /′ ^x ⟧ c)
-  → ⪧′ Γ ⊨′ `^x ⋅ e1 & e2 ⇒′ c
+      ⊨′ F ⇒′ ex_subst_cont F x c)
+  → ⪧′ Γ ⊨′ `^x ⇒′ c
 
 (* general reduce *)
 | st_gred : forall Γ A B c
   , A ⟶′ B
-  → ⪧′ Γ ⫢′ c $′ B
+  → ⪧′ Γ ⊨′ c $′ B
   → ⪧′ Γ ⊨′ A ⟼′ c
 | st_gred_forall : forall L Γ A B c
   , (forall x, x `notin` L
@@ -362,27 +383,30 @@ Inductive wl_step : worklist -> Prop :=
 
 (* kind ex infer *)
 | st_kv_eq : forall Γ x c
-  , ⪧′ ⟦ak_star /′ ⧼x⧽⟧ Γ ⫢′ ⟦ak_star /′ ⧼x⧽⟧ c $′ ◻′
+  , ⪧′ ⟦ak_star /′ ⧼x⧽⟧ Γ ⊨′ k_subst_cont ak_star x c $′ ◻′
   → ⪧′ Γ ⊨′ ⧼`^x⧽ <: ⧼`^x⧽ ⇒′ c
 | st_kv_lr : forall Γ x y c
   , x <> y
   → ⪧′ ⟦ak_star /′ ⧼y⧽⟧ ⟦ak_star /′ ⧼x⧽⟧ Γ
-    ⫢′ ⟦ak_star /′ ⧼y⧽⟧ ⟦ak_star /′ ⧼x⧽⟧ c $′ ◻′
+    ⊨′ k_subst_cont ak_star y (k_subst_cont ak_star x c) $′ ◻′
   → ⪧′ Γ ⊨′ ⧼`^x⧽ <: ⧼`^y⧽ ⇒′ c
 | st_kv_l : forall Γ x c
-  , ⪧′ ⟦ak_star /′ ⧼x⧽⟧ Γ ⫢′ ⟦ak_star /′ ⧼x⧽⟧ c $′ ◻′
+  , ⪧′ ⟦ak_star /′ ⧼x⧽⟧ Γ ⊨′ k_subst_cont ak_star x c $′ ◻′
   → ⪧′ Γ ⊨′ ⧼`^x⧽ <: ⋆′ ⇒′ c
 | st_kv_r : forall Γ x c
-  , ⪧′ ⟦ak_star /′ ⧼x⧽⟧ Γ ⫢′ ⟦ak_star /′ ⧼x⧽⟧ c $′ ◻′
+  , ⪧′ ⟦ak_star /′ ⧼x⧽⟧ Γ ⊨′ k_subst_cont ak_star x c $′ ◻′
   → ⪧′ Γ ⊨′ ⋆′ <: ⧼`^x⧽ ⇒′ c
 
 (* check *)
 | st_check : forall Γ e1 e2 b A
-  , ⪧′ Γ ,?′ b ⊨′ e1 <: e2 ⇒′ ⦃ ↑′ 0 ≲′ A ⦄
+  , ⪧′ Γ ,?′ b ⊨′ e1 <: e2 ⇒′ c_check A
   → ⪧′ Γ ⊨′ b ⊢? e1 <: e2 ⇐′ A
 | st_comp_box_l : forall Γ k
   , ⪧′ ⟦ ak_box /′ ⧼k⧽ ⟧ Γ
-  (*  (wl_step (wl_work Γ (w_compact (ae_kind ak_box) (ae_ex k))))) *)
+  (*
+     why notation?
+     (wl_step (wl_work Γ (w_compact (ae_kind ak_box) (ae_ex k)))))
+  *)
   → ⪧′ Γ ⊨′ ◻′ ≲′ ⧼`^k⧽
 | st_comp_box_r : forall Γ k
   , ⪧′ ⟦ ak_box /′ ⧼k⧽ ⟧ Γ
@@ -398,7 +422,11 @@ Inductive wl_step : worklist -> Prop :=
 | st_comp_sub : forall L Γ A B
   , (forall k, k `notin` L → ⪧′ Γ,′ ⧼^k⧽ ⊨′ A <: B ⇐′ ⧼`^k⧽)
   → ⪧′ Γ ⊨′ A ≲′ B
-
+(* TODO: apply continuation *)
+| st_app_cont : forall Γ c e Γ'
+  , apply_cont c e Γ'
+  → ⪧′ Γ ⫢′ Γ'
+  → ⪧′ Γ ⊨′ c $′ e
 (* elim bindings *)
 | st_bind_var : forall L Γ x A
   , (forall k, k `notin` L → ⪧′ Γ ,′ ⧼^k⧽ ⊨′ A ⇐′ ⧼`^k⧽)
